src/Init/Data/Option/Lemmas.lean
@@ -12,12 +12,12 @@ import Init.Ext
 
 namespace Option
 
--- @[deprecated mem_def (since := "2025-04-07")]
--- theorem mem_iff {a : α} {b : Option α} : a ∈ b ↔ b = some a := .rfl
+@[deprecated mem_def (since := "2025-04-07")]
+theorem mem_iff {a : α} {b : Option α} : a ∈ b ↔ b = some a := .rfl
 
--- theorem mem_some {a b : α} : a ∈ some b ↔ b = a := by simp
+theorem mem_some {a b : α} : a ∈ some b ↔ b = a := by simp
 
--- theorem mem_some_self (a : α) : a ∈ some a := mem_some.2 rfl
+theorem mem_some_self (a : α) : a ∈ some a := rfl
 
 theorem some_ne_none (x : α) : some x ≠ none := nofun
 
@@ -29,13 +29,16 @@ protected theorem «exists» {p : Option α → Prop} :
   ⟨fun | ⟨none, hx⟩ => .inl hx | ⟨some x, hx⟩ => .inr ⟨x, hx⟩,
    fun | .inl h => ⟨_, h⟩ | .inr ⟨_, hx⟩ => ⟨_, hx⟩⟩
 
--- theorem get_mem : ∀ {o : Option α} (h : isSome o), o.get h ∈ o
---   | some _, _ => rfl
+theorem get_mem : ∀ {o : Option α} (h : isSome o), o.get h ∈ o
+  | some _, _ => rfl
 
--- theorem get_of_mem : ∀ {o : Option α} (h : isSome o), a ∈ o → o.get h = a
---   | _, _, rfl => rfl
+theorem get_of_mem : ∀ {o : Option α} (h : isSome o), a ∈ o → o.get h = a
+  | _, _, rfl => rfl
 
--- @[simp] theorem not_mem_none (a : α) : a ∉ (none : Option α) := nofun
+theorem get_of_eq_some : ∀ {o : Option α} (h : isSome o), o = some a → o.get h = a
+  | _, _, rfl => rfl
+
+@[simp] theorem not_mem_none (a : α) : a ∉ (none : Option α) := nofun
 
 theorem getD_of_ne_none {x : Option α} (hx : x ≠ none) (y : α) : some (x.getD y) = x := by
   cases x; {contradiction}; rw [getD_some]
@@ -69,8 +72,11 @@ theorem get_inj {o1 o2 : Option α} {h1} {h2} :
   match o1, o2, h1, h2 with
   | some a, some b, _, _ => simp only [Option.get_some, Option.some.injEq]
 
--- theorem mem_unique {o : Option α} {a b : α} (ha : a ∈ o) (hb : b ∈ o) : a = b :=
---   some.inj <| ha ▸ hb
+theorem mem_unique {o : Option α} {a b : α} (ha : a ∈ o) (hb : b ∈ o) : a = b :=
+  some.inj <| ha ▸ hb
+
+theorem eq_some_unique {o : Option α} {a b : α} (ha : o = some a) (hb : o = some b) : a = b :=
+  some.inj <| ha ▸ hb
 
 @[ext] theorem ext : ∀ {o₁ o₂ : Option α}, (∀ a, o₁ = some a ↔ o₂ = some a) → o₁ = o₂
   | none, none, _ => rfl
@@ -82,16 +88,16 @@ set_option Elab.async false
 theorem eq_none_iff_forall_ne_some : o = none ↔ ∀ a, o ≠ some a := by
   cases o <;> simp
 
--- theorem eq_none_iff_forall_not_mem : o = none ↔ ∀ a, a ∉ o :=
---   eq_none_iff_forall_not_eq_some
+theorem eq_none_iff_forall_not_mem : o = none ↔ ∀ a, a ∉ o :=
+  eq_none_iff_forall_ne_some
 
 theorem isSome_iff_exists : isSome x ↔ ∃ a, x = some a := by cases x <;> simp [isSome]
 
 theorem isSome_eq_isSome : (isSome x = isSome y) ↔ (x = none ↔ y = none) := by
   cases x <;> cases y <;> simp
 
--- theorem isSome_of_mem {x : Option α} {y : α} (h : y ∈ x) : x.isSome := by
---   cases x <;> trivial
+theorem isSome_of_mem {x : Option α} {y : α} (h : y ∈ x) : x.isSome := by
+  cases x <;> trivial
 
 theorem isSome_of_eq_some {x : Option α} {y : α} (h : x = some y) : x.isSome := by
   cases x <;> trivial
@@ -155,9 +161,9 @@ theorem bind_eq_none' {o : Option α} {f : α → Option β} :
     o.bind f = none ↔ ∀ b a, o = some a → f a ≠ some b := by
   cases o <;> simp [eq_none_iff_forall_ne_some]
 
--- theorem mem_bind_iff {o : Option α} {f : α → Option β} :
---     b ∈ o.bind f ↔ ∃ a, a ∈ o ∧ b ∈ f a := by
---   cases o <;> simp
+theorem mem_bind_iff {o : Option α} {f : α → Option β} :
+    b ∈ o.bind f ↔ ∃ a, a ∈ o ∧ b ∈ f a := by
+  cases o <;> simp
 
 theorem bind_comm {f : α → β → Option γ} (a : Option α) (b : Option β) :
     (a.bind fun x => b.bind (f x)) = b.bind fun y => a.bind fun x => f x y := by
@@ -256,7 +262,7 @@ theorem comp_map (h : β → γ) (g : α → β) (x : Option α) : x.map (h ∘ 
 @[simp] theorem map_comp_map (f : α → β) (g : β → γ) :
     Option.map g ∘ Option.map f = Option.map (g ∘ f) := by funext x; simp
 
--- theorem mem_map_of_mem (g : α → β) (h : a ∈ x) : g a ∈ Option.map g x := h.symm ▸ map_some' ..
+theorem mem_map_of_mem (g : α → β) (h : a ∈ x) : g a ∈ Option.map g x := h.symm ▸ map_some' ..
 
 theorem map_inj_right {f : α → β} {o o' : Option α} (w : ∀ x y, f x = f y → x = y) :
     o.map f = o'.map f ↔ o = o' := by
@@ -304,9 +310,9 @@ abbrev isSome_filter_of_isSome := @isSome_of_isSome_filter
       rintro rfl
       simpa using h
 
--- theorem mem_filter_iff {p : α → Bool} {a : α} {o : Option α} :
---     a ∈ o.filter p ↔ a ∈ o ∧ p a := by
---   simp
+theorem mem_filter_iff {p : α → Bool} {a : α} {o : Option α} :
+    a ∈ o.filter p ↔ a ∈ o ∧ p a := by
+  simp
 
 theorem filter_eq_bind (x : Option α) (p : α → Bool) :
     x.filter p = x.bind (Option.guard (fun a => p a)) := by
@@ -376,8 +382,8 @@ theorem join_map_eq_map_join {f : α → β} {x : Option (Option α)} :
 theorem join_join {x : Option (Option (Option α))} : x.join.join = (x.map join).join := by
   cases x <;> simp
 
--- theorem mem_of_mem_join {a : α} {x : Option (Option α)} (h : a ∈ x.join) : some a ∈ x :=
---   h.symm ▸ join_eq_some.1 h
+theorem mem_of_mem_join {a : α} {x : Option (Option α)} (h : a ∈ x.join) : some a ∈ x :=
+  h.symm ▸ join_eq_some.1 h
 
 @[simp] theorem some_orElse (a : α) (x : Option α) : (some a <|> x) = some a := rfl
 
@@ -651,21 +657,21 @@ section ite
     some a = (if p then b else none) ↔ p ∧ some a = b := by
   split <;> simp_all
 
--- theorem mem_dite_none_left {x : α} {_ : Decidable p} {l : ¬ p → Option α} :
---     (x ∈ if h : p then none else l h) ↔ ∃ h : ¬ p, x ∈ l h := by
---   simp
+theorem mem_dite_none_left {x : α} {_ : Decidable p} {l : ¬ p → Option α} :
+    (x ∈ if h : p then none else l h) ↔ ∃ h : ¬ p, x ∈ l h := by
+  simp
 
--- theorem mem_dite_none_right {x : α} {_ : Decidable p} {l : p → Option α} :
---     (x ∈ if h : p then l h else none) ↔ ∃ h : p, x ∈ l h := by
---   simp
+theorem mem_dite_none_right {x : α} {_ : Decidable p} {l : p → Option α} :
+    (x ∈ if h : p then l h else none) ↔ ∃ h : p, x ∈ l h := by
+  simp
 
--- theorem mem_ite_none_left {x : α} {_ : Decidable p} {l : Option α} :
---     (x ∈ if p then none else l) ↔ ¬ p ∧ x ∈ l := by
---   simp
+theorem mem_ite_none_left {x : α} {_ : Decidable p} {l : Option α} :
+    (x ∈ if p then none else l) ↔ ¬ p ∧ x ∈ l := by
+  simp
 
--- theorem mem_ite_none_right {x : α} {_ : Decidable p} {l : Option α} :
---     (x ∈ if p then l else none) ↔ p ∧ x ∈ l := by
---   simp
+theorem mem_ite_none_right {x : α} {_ : Decidable p} {l : Option α} :
+    (x ∈ if p then l else none) ↔ p ∧ x ∈ l := by
+  simp
 
 @[simp] theorem isSome_dite {p : Prop} {_ : Decidable p} {b : p → β} :
     (if h : p then some (b h) else none).isSome = true ↔ p := by
